1. What is an arithmetic sequence?

- A sequence where each term is a product of the previous term
- A dequence where each term is the sum of all previous terms
- A sequence where each term is divided by a constant
- A sequence where each term is obtained by adding a constant to the previous term. `Correct`

2. Which term represents the common difference in an arithmetic sequence

- r
- d `correct`
- n
- a

3. What is the first term of an arithmetic sequence called?

- d
- a `correct`
- r
- n

4. How is the nth term of an arithmetic sequence represented?

- a + nd
- a + (n-1)^d^ `correct`
- a / (n-1)
- a \* r ^(n-1)^

5. What is a geometric sequence

- A sequence where each term is divided by a constant
- A sequence where each term is added by a constant
- A sequence where each term is multiplied by a constant `correct`
- A sequence where each term is subtracteed by a constant

6. What does the common ratio in a geometric sequnce represent

- The product of terms
- The sum of terms
- The ratio between consecutive terms `correct`
- The difference between terms

7. How is the nth term of a geometric sequence represented?

- a \* (n-1)
- a + (n-1)d
- a / r^(n-1)^ `correct`
- a \* r^(n-1)^

8. What happens to a geometric sequence if the common ratio `r` is greater than 1?

- It remains constant
- It oscillates between values
- it diverges to infinity `diverges to infinity`
- It converges to a number

9. What is a Fibonacci sequence?

- A sequence where each term is the quotient of the two preceding terms
- A sequence where each term is the product of the two preceeding terms
- A sequence where each term is the sum of the two preceeding terms `Correct`
- A sequence whre each term is the difference of the two preciding terms

10. Find the 10th term of an arithmetic sequence where the first term `a` is 5 and the common difference `d` is 3.

<details>
  <summary>Solution to question 10</summary>

To find the 10th term of the arithmetic sequence, we use the formula for the nth term of an arithmetic sequence:

a~n~ = a~1~ + (n - 1)\* d

`Given:`

- First term a~1~ = 5
- Common difference `d` = 3
- `n` = 10 (the term we need to find)

`Substituting the values into the formula:`

a~10~ = 5 + (10 - 1) x 3
a~10~ = 5 + 9 x 3
a~10~ = 5 + 27
a~10~ = 32

`Final Answer:`

The 10th term of the arithmetic sequence is **32**.

</details>

<br>

11. Determine the 5th term of a geometric sequence where the first term `a` is 2 and the coomon ration `r` is 3

<details>
  <summary>Solution to question 11</summary>

To find the 5th term (a~5~) of a geometric sequence, we use the formula for the nth term:

a~n~ = a~1~ x r ^n-1^

`Given:`

- a~1~ = 2 (first term)
- `r` = 3 (common ratio)
- `n` = 5 (we need to find the 5th term)

`Substituting the values into the formula:`

a~5~ = 2 x 3 ^5-1^
a~5~ = 2 x 3 ^4^
a~5~ = 2 x 81
a~5~ = 162

`Final Answer:`

The 5th term of the geometric sequnece is 162.

</details>

<br>

12. If the 4th term of an arithmetic sequence is 20 and the common difference `d` is 5, find the first term `a`

<details>
  <summary>Solution to question 12</summary>

To find the first term a~1~ of the arithmetic sequence, we use the formula for the n-th term of an arithmetic sequence:

a~n~ = a~1~ + (n - 1) x d

`Given:`

- The 4th term a~4~ = 20,
- The common difference d = 5,
- We need to find a~1~, the first term.

`Step-by-step solution:`

The formula for the 4th term (a~4~) is:

a~4~ = a~1~ + (4 - 1) x d
20 = a~1~ + 3 x 5
20 = a~1~ + 15

Now, solve for a~1~:

a~1~ = 20 - 15
a~1~ = 5

`Final Answer:`

The first term of the arithmetic sequence is **5**.

</details>

<br>

13. Calculate the sum of the first 6 terms of an arithmetic sequence with `a` = 2 and `d` = 4

<details>
  <summary>Solution to question 13</summary>

To calculate the sum of the first 6 terms of an arithmetic sequence, we use the formula for the sum of the first `n` terms of an arithmetic sequence:

S~n~ = n/2 x (a~1~ + a~n~)

`Where`:

- S~n~ is the sum of the first n terms
- n is number of terms
- a~1~ is the first term
- a~n~ is the n-th term

`Given:`

- First term a~1~ = 2
- Common difference d = 4
- Number of terms n = 6

Step 1: Find the 6th term (a~6~) using the formula for the n-th term:

a~n~ = a~1~ + (n-1) x d

Substitute a~1~ = 2, d = 4, n = 6

a~6~ = 2 + (6-1)x4
a~6~ = 2 + 5 x 4 = 2 + 20 = 22

Step 2: Use the sum formula to find S~6~

S~6~ = $\frac{6}{2}$ x (2 + 22)
S~6~ = 3 x 24 = 72

`Final Answer:`

The sum of the first 6 term of the arithmetic sequence is 72

</details>

<br>

14.Find the sum of the first four terms of a geometric sequence where `a` = 1 and `r` = 2

<details>
  <summary>Solution to question 14</summary>

To find the sum of the first 4 terms of a geometric sequence, we use the formula for the sum of the first n terms of a geometric sequence:

S~n~ = a~1~ x $\frac{1-r^2}{1-r}$ for r $\not=$ 1

`Where`:

- S~n~ is the sum of the first n terms
- n is number of terms
- a~1~ is the first term
- a~n~ is the n-th term

`Given:`

- a~1~ = 1
- r = 2
  n = 4

Step 1: Substitute the given values into the sum formula:

S~4~ = 1 x $\frac{1-2^4}{1-2}$
S~4~ = $\frac{1-16}{1-2}$
S~4~ = $\frac{-15}{-1}$
S~4~ = 15

`Final Answer:`

The sum of the first 4 terms of the geometric sequence is 15.

</details>

<br>

15. Determine the sixth term of a Fibonachi sequence starting with u~1~ = 0 and u~2~ = 1
