### Exponential functions

**1. For the exponential function a^x^, if a = $\frac{1}{2}$, which of the following statements is true as _x_ approaches infinity?**

- The function oscillates between positive and negative values
- The function approaches infinity
- The function remains constant
- The function approaches zero

<details>
  <summary>Solution</summary>

The given function is:

\[
f(x) = \left(\frac{1}{2}\right)^x
\]

Step 1: Understand the behavior of the function

- The base \( a = \frac{1}{2} \) is between 0 and 1.
- Exponential functions with bases in the range \( 0 < a < 1 \) decrease as \( x \) increases.

Step 2: Analyze the limit as \( x \to \infty \)

- As \( x \) grows larger, the exponentiation \( \left(\frac{1}{2}\right)^x \) results in smaller and smaller values.
- Mathematically,

  \[
  \lim\_{x \to \infty} \left(\frac{1}{2}\right)^x = 0.
  \]

Thus, the function approaches **zero**.

Step 3: Eliminate incorrect choices

- The function does **not** oscillate because it is always positive.
- The function does **not** approach infinity; instead, it decreases.
- The function does **not** remain constant since its value decreases continuously.

Correct Answer:
**The function approaches zero.**

</details>

</br>

**2. Which property of exponential functions is illustrated by the equation a^n^ x a^m^ = a^n+m^**

- Division property
- Multiplication property
- Negative exponent property
- Power of a power property

<details>
  <summary>Solution</summary>

The given equation is:

\[
a^n \times a^m = a^{n+m}
\]

Step 1: Identify the property

- This equation states that when multiplying two exponential expressions with the **same base**, the exponents are **added**.
- This is a fundamental property of exponentiation.

Step 2: Match with the given answer choices

- **Division property**: This deals with the rule \(\frac{a^n}{a^m} = a^{n-m}\), which is not applicable here.
- **Multiplication property**: This correctly describes how exponents add when multiplying powers of the same base.
- **Negative exponent property**: This applies when exponents are negative, e.g., \( a^{-n} = \frac{1}{a^n} \), which is not relevant here.
- **Power of a power property**: This applies when an exponent is raised to another exponent, e.g., \( (a^n)^m = a^{n \cdot m} \), which is different from the given equation.

Correct Answer:
**Multiplication property**

</details>

</br>

**3. What is the result of $(16)^{\frac{3}{4}}$**

- 2
- 8
- 16
- 4

<details>
  <summary>Solution</summary>

We need to evaluate:

\[
(16)^{\frac{3}{4}}
\]

Step 1: Express 16 as a Power of 2

\[
16 = 2^4
\]

Rewriting the expression:

\[
(2^4)^{\frac{3}{4}}
\]

Step 2: Use the Power of a Power Property

\[
(a^m)^n = a^{m \cdot n}
\]

Applying this property:

\[
2^{4 \times \frac{3}{4}} = 2^{3}
\]

Step 3: Compute the Exponentiation

\[
2^3 = 8
\]

Correct Answer:

**8**

</details>

</br>

4. **If f~1~(x) = 2^x^ and f~2~(x) = $({\frac{1}{2}})^x$, what is the relationship between f~1~(x) and f~2~(x)**.

- f~1~(x) = f~2~(-x)
- f~1~(-x) = f~2~(-x)
- f~1~(x) = f~2~(x)
- f~1~(x) = f~2~(x)

<details>
  <summary>Solution</summary>

We are given the functions:

\[
f_1(x) = 2^x
\]

\[
f_2(x) = \left(\frac{1}{2}\right)^x
\]

Step 1: Rewrite \( f_2(x) \)

We express \( f_2(x) \) using exponent properties:

\[
f_2(x) = \left(\frac{1}{2}\right)^x = 2^{-x}
\]

Step 2: Compare \( f_1(x) \) and \( f_2(x) \)

From the above expressions, we see:

\[
f_2(x) = 2^{-x}
\]

which means:

\[
f_1(-x) = 2^{-x} = f_2(x)
\]

or equivalently:

\[
f_1(x) = f_2(-x)
\]

Conclusion:

Thus, the correct answer is:

\[
\mathbf{f_1(x) = f_2(-x)}
\]

</details>

</br>

5. **Solve the x in the equation 3^2x^ = 27**

<details>
  <summary>Solution</summary>

We are given the equation:

\[
3^{2x} = 27
\]

Step 1: Express 27 as a Power of 3
Since \( 27 = 3^3 \), we rewrite the equation as:

\[
3^{2x} = 3^3
\]

Step 2: Equating the Exponents
Since the bases are the same, we set the exponents equal to each other:

\[
2x = 3
\]

Step 3: Solve for \( x \)

\[
x = \frac{3}{2}
\]

Final Answer:
\[
\mathbf{x = \frac{3}{2}}
\]

</details>

</br>

6. **Find the value of y if $ y = 2^{\frac{5}{3}} $**

<details>
  <summary>Solution</summary>

We are given the equation:

\[
y = 2^{\frac{5}{3}}
\]

Step 1: Rewrite the Exponentiation

The exponent \(\frac{5}{3}\) can be broken down as:

\[
2^{\frac{5}{3}} = \left(2^{\frac{1}{3}}\right)^5
\]

This means we first calculate \(2^{\frac{1}{3}}\), which is the **cube root of 2**.

Step 2: Compute \( 2^{\frac{1}{3}} \)

The cube root of 2 is:

\[
2^{\frac{1}{3}} \approx 1.2599
\]

Step 3: Raise the Result to the Power of 5

Now, we compute:

\[
(1.2599)^5
\]

Using exponentiation:

\[
1.2599^5 \approx 3.1748
\]
Step 4: Final Answer

\[
y \approx 3.175
\]

So, the approximate value of \( y = 2^{\frac{5}{3}} \) is **3.175** (rounded to three decimal places).

</details>

</br>

7. **Verify the property a^-n^ = ${\frac{1}{a^n}} $ by using a = 2 and n = 3**

<details>
  <summary>Solution</summary>

Let's verify the property again:

\[
a^{-n} = \frac{1}{a^n}
\]

#iven:

- \( a = 2 \)
- \( n = 3 \)

Step 1: Compute the Left-Hand Side (LHS)

\[
2^{-3} = \frac{1}{2^3}
\]

Step 2: Compute the Right-Hand Side (RHS)

\[
\frac{1}{2^3} = \frac{1}{8} = 0.125
\]

Step 3: Compare Both Sides

\[
2^{-3} = 0.125, \quad \frac{1}{2^3} = 0.125
\]

Since both sides are equal, the property holds true:

\[
a^{-n} = \frac{1}{a^n}
\]

</details>

</br>

8. **If a = 16 and n = ${\frac{3}{4}}$, find the value of a^n^**

<details>
  <summary>Solution</summary>

We are given:

\[
a = 16, \quad n = \frac{3}{4}
\]

We need to compute:

\[
a^n = 16^{\frac{3}{4}}
\]

Step 1: Rewrite the Exponent
\[
16^{\frac{3}{4}} = \left(16^{\frac{1}{4}}\right)^3
\]

This means we first calculate \( 16^{\frac{1}{4}} \), which is the **fourth root of 16**.

Step 2: Compute \( 16^{\frac{1}{4}} \)
\[
16^{\frac{1}{4}} = \sqrt[4]{16} = 2
\]

Step 3: Raise the Result to the Power of 3
\[
2^3 = 8
\]

Step 4: Final Answer
\[
16^{\frac{3}{4}} = 8
\]

Thus, the value of \( a^n \) is **8**.

</details>

</br>

9. **Determine y if y = $4^{-\frac{1}{2}}$**
