### Further differentiation 1

##### 1. What does the f'(x) represent in the differentiation?

- The integral of the function
- The value of the function at x
- The average rate of the change between two points
- The slope of the tangent line at x

<details>
  <summary>Solution</summary>

The correct answer is:

**The slope of the tangent line at x**

\( f'(x) \) represents the **instantaneous rate of change** of the function at \( x \), which is the **slope of the tangent line** to the curve at that point.

  </br>

</details>

</br>

##### 2. Which of the following expressions defines the derivative of f(x) using limits?

- lim~h->0~ ${\frac{f(x+h) - f(x)}{h}}$
- lim~h->0~ ${\frac{f(x) - f(x-h)}{h}}$
- lim~h->0~ ${\frac{f(x+h) - f(x-h)}{h}}$
- lim~h->0~ ${\frac{f(x+h) - f(x-h)}{2h}}$

details>

  <summary>Solution</summary>

The correct answer is:

**\(\lim\_{{h \to 0}} \frac{f(x+h) - f(x)}{h}\)**

This is the **definition of the derivative** of \( f(x) \) using limits. It represents the **instantaneous rate of change** of \( f(x) \) at \( x \), which is also the slope of the tangent line to the curve at that point.

Explanation of the other options:

- **\(\lim\_{{h \to 0}} \frac{f(x) - f(x-h)}{h}\)**:

  - This is similar to the correct definition but written in terms of backward differences. It is not the standard definition.

- **\(\lim\_{{h \to 0}} \frac{f(x+h) - f(x-h)}{h}\)**:

  - This expression is incorrect because it does not properly take the limit as \( h \to 0 \) in the standard form.

- **\(\lim\_{{h \to 0}} \frac{f(x+h) - f(x-h)}{2h}\)**:
  - This is the **symmetric difference quotient**, an approximation for the derivative, but not its exact definition.

Thus, the first option is the correct definition of the derivative using limits. ðŸš€

  </br>

</details>

</br>

##### 3. If f(x) = x^3^, what is f;(x)?

- 3x^2^
- 3x
- x^3^
- x^2^

<details>
  <summary>Solution</summary>

Given the function:
\[
f(x) = x^3
\]

To find \( f'(x) \), we use the **power rule** of differentiation:

\[
\frac{d}{dx} x^n = n x^{n-1}
\]

Applying this rule:

\[
f'(x) = 3x^{3-1} = 3x^2
\]

Correct Answer:

âœ… **3xÂ²**

  </br>

</details>

</br>

##### 4. What technique is used to find the derivative of f(x) = x^2^ from first principles?

- Binomial expansion
- Quotient rule
- Product rule
- Integration by parts

<details>
  <summary>Solution</summary>

The correct answer is:

âœ… **Binomial expansion**

### Explanation:

To find the derivative of \( f(x) = x^2 \) **from first principles**, we use the **definition of the derivative**:

\[
f'(x) = \lim\_{{h \to 0}} \frac{f(x+h) - f(x)}{h}
\]

Substituting \( f(x) = x^2 \):

\[
f'(x) = \lim\_{{h \to 0}} \frac{(x+h)^2 - x^2}{h}
\]

Expanding \( (x+h)^2 \) using **binomial expansion**:

\[
(x+h)^2 = x^2 + 2xh + h^2
\]

Now, substitute back:

\[
f'(x) = \lim\_{{h \to 0}} \frac{x^2 + 2xh + h^2 - x^2}{h}
\]

\[
= \lim\_{{h \to 0}} \frac{2xh + h^2}{h}
\]

Factor out \( h \):

\[
= \lim\_{{h \to 0}} (2x + h)
\]

As \( h \to 0 \), we get:

\[
f'(x) = 2x
\]

### Why the other options are incorrect:

- **Quotient Rule**: Used for functions of the form \( \frac{f(x)}{g(x)} \), which is not applicable here.
- **Product Rule**: Used when differentiating a product of two functions, but \( x^2 \) is a single function.
- **Integration by Parts**: This is an integration technique, not differentiation.

Thus, **binomial expansion** is the correct technique when differentiating \( f(x) = x^2 \) from first principles. ðŸš€e

  </br>

</details>

</br>

##### 5. Which of the following expressions is the derivative of f(x) = x^2^ using the limit definition?

- lim~Î”x\_>0~ ${\frac{(x+Î”x)^3 -x^3}{Î”x}}$
- lim~Î”x\_>0~ ${\frac{(x^2 - (z-Î”x)^2}{Î”x}}$
- lim~Î”x\_>0~ ${\frac{((x+Î”x)-x}{Î”x}}$
- lim~Î”x\_>0~ ${\frac{(x+Î”)^2}{Î”x}}$

<details>
  <summary>Solution</summary>

The correct expression that represents the derivative of \( f(x) = x^2 \) using the **limit definition of a derivative** is:

âœ…
\[
\lim\_{\Delta x \to 0} \frac{(x+\Delta x)^2 - x^2}{\Delta x}
\]

However, none of the given options seem to be exactly correct. Let's analyze them:

1. **\(\lim\_{\Delta x \to 0} \frac{(x+\Delta x)^3 - x^3}{\Delta x}\)**

   - Incorrect. This is the derivative definition for \( f(x) = x^3 \), not \( x^2 \).

2. **\(\lim\_{\Delta x \to 0} \frac{x^2 - (z-\Delta x)^2}{\Delta x}\)**

   - Incorrect. This does not match the standard limit definition of the derivative.

3. **\(\lim\_{\Delta x \to 0} \frac{( (x+\Delta x) - x )}{\Delta x}\)**

   - Incorrect. This simplifies to \( \frac{\Delta x}{\Delta x} = 1 \), which is not the derivative of \( x^2 \).

4. **\(\lim\_{\Delta x \to 0} \frac{(x+\Delta)^2}{\Delta x}\)**
   - Incorrect. It should be **\(\frac{(x+\Delta x)^2 - x^2}{\Delta x}\)** instead.

Correct Limit Definition for \( f(x) = x^2 \):

\[
f'(x) = \lim\_{\Delta x \to 0} \frac{(x+\Delta x)^2 - x^2}{\Delta x}
\]

Expanding \( (x+\Delta x)^2 \) using binomial expansion:

\[
= \lim\_{\Delta x \to 0} \frac{x^2 + 2x\Delta x + (\Delta x)^2 - x^2}{\Delta x}
\]

\[
= \lim\_{\Delta x \to 0} \frac{2x\Delta x + (\Delta x)^2}{\Delta x}
\]

\[
= \lim\_{\Delta x \to 0} (2x + \Delta x)
\]

\[
= 2x
\]

Thus, **\( f'(x) = 2x \)**, but none of the answer choices match the correct limit definition exactly. If you have a formatting issue in your options, check for a choice similar to:

\[
\lim\_{\Delta x \to 0} \frac{(x+\Delta x)^2 - x^2}{\Delta x}
\]

  </br>

</details>

</br>
