## Midterm

`Question 1 (A)`

Given:

(P∨Q)→R and (P→R)∧(Q→R)
Claim: They are logically equivalent.

Proof:

(⇒ direction):

Assume (P∨Q)→R.

If P is true, then P ∨ Q is true → R is true → P → R holds.
If Q is true, then P ∨ Q is true → R is true → Q → R holds.

So, (P→R)∧(Q→R).

(⇐ direction):

Assume ( P → R ) ∧ ( Q → R).

If P ∨ Q is true, then either Q is true.
If P, then R (since P → R)
if Q, then R

So,

( P ∨ Q ) → R holds.

`Question 1 (B)`

A, C, and D are tautologies.

`Question 1 (C)`

P → ( Q → R ) ≡ P → ( ¬ Q ∨ R ) ≡ ¬ P ∨ ¬ Q ∨ R ≡ ¬ ( P ∧ Q ) ∨ R ≡( P ∧ Q ) → R

So both expressions are logically equivalent.
