### Differentiating polynomials

##### 1. What is the derivative of the function f(x) = 3x^4^

- 9x^3^
- 12x^3^
- 4x^3^
- 6x^3^

<details>
  <summary>Solution</summary>

To find the derivative of \( f(x) = 3x^4 \), we use the **power rule**:

\[
\frac{d}{dx} [ax^n] = a \cdot n x^{n-1}
\]

**Step 1: Identify Constants**

- \( a = 3 \)
- \( n = 4 \)

**Step 2: Differentiate**

\[
f'(x) = 3 \cdot 4x^{4-1}
\]

\[
f'(x) = 12x^3
\]

**Final Answer:**

‚úÖ **12x¬≥**

Thus, the correct answer is:
**\( \mathbf{12x^3} \)** üéØ

  </br>

</details>

</br>

##### 2. Which of the following represents the derivative of f(x) = sin(x)?

- -cos(x)
- -sin(x)
- tan(x)
- cos(x)

<details>
  <summary>Solution</summary>

To differentiate \( f(x) = \sin(x) \), we use the standard derivative rule:

\[
\frac{d}{dx} \sin(x) = \cos(x)
\]

**Step 1: Identify the Function**

Given:
\[
f(x) = \sin(x)
\]

**Step 2: Apply the Derivative Rule**

\[
f'(x) = \cos(x)
\]

**Final Answer:**

‚úÖ **cos(x)**

Thus, the correct choice is:
**\( \mathbf{\cos(x)} \)** üéØ

  </br>

</details>

</br>

##### 3. If f(x) = e^x^, what is f'(x)

- e^x^
- xe^x-1^
- e^x-1^
- xe^x^

<details>
  <summary>Solution</summary>

To differentiate \( f(x) = e^x \), we use the fundamental rule:

\[
\frac{d}{dx} e^x = e^x
\]

**Step 1: Identify the Function**
\[
f(x) = e^x
\]

**Step 2: Differentiate**
\[
f'(x) = e^x
\]
**Final Answer:**
‚úÖ **\( e^x \)**

Thus, the correct choice is:
**\( \mathbf{e^x} \)** üéØ

  </br>

</details>

</br>

##### 4. Find the derivative of f(x) = x^2^ - 3x + 5

- 2x - 3
- 2x - 3x + 5
- 2x + 3
- 2x - 3 + 5

<details>
  <summary>Solution</summary>

To differentiate \( f(x) = x^2 - 3x + 5 \), we apply the **power rule** and the derivative of a constant:

**Step 1: Differentiate Each Term**

1. \( \frac{d}{dx} x^2 = 2x \)
2. \( \frac{d}{dx} (-3x) = -3 \)
3. \( \frac{d}{dx} (5) = 0 \) (since the derivative of a constant is 0)

**Step 2: Combine the Results**

\[
f'(x) = 2x - 3
\]

**Final Answer:**

‚úÖ **2x - 3**

Thus, the correct choice is:
**\( \mathbf{2x - 3} \)** üéØ

  </br>

</details>

</br>

##### 5. Which statement is true about the derivative of a constant function?

- The derivative is one
- The derivative does not exist
- The derivative is the constant itself
- The derivative is zero

<details>
  <summary>Solution</summary>

The correct answer is:

‚úÖ **The derivative is zero**

**Explanation:**

For a constant function \( f(x) = c \) (where \( c \) is a constant), the derivative is given by:

\[
\frac{d}{dx} (c) = 0
\]

This is because a constant function does not change, so its **rate of change (slope)** is always **zero**.

**Why the other options are incorrect:**

- **"The derivative is one"** ‚ùå ‚Üí Incorrect because a constant function has no change, so the derivative is **not 1**.
- **"The derivative does not exist"** ‚ùå ‚Üí Incorrect because the derivative of a constant **does exist**, and it is **0**.
- **"The derivative is the constant itself"** ‚ùå ‚Üí Incorrect because the derivative of a constant is **not the constant itself**, but rather **zero**.

**Final Conclusion:**

For any constant function \( f(x) = c \),
**\( f'(x) = 0 \)** üöÄ

  </br>

</details>

</br>

##### 6. Find the derivative of the function f(x) = 4x^3^ - 5x^2^ + 6x - 7

<details>
  <summary>Solution</summary>

Let's differentiate the function **\( f(x) = 4x^3 - 5x^2 + 6x - 7 \)** again, step by step.

**Step 1: Apply the Power Rule**
The **power rule** states:

\[
\frac{d}{dx} x^n = n x^{n-1}
\]

Now, we differentiate each term separately:

1. **Differentiate \( 4x^3 \)**:
   \[
   \frac{d}{dx} (4x^3) = 4 \cdot 3x^{3-1} = 12x^2
   \]
2. **Differentiate \( -5x^2 \)**:
   \[
   \frac{d}{dx} (-5x^2) = -5 \cdot 2x^{2-1} = -10x
   \]
3. **Differentiate \( 6x \)**:
   \[
   \frac{d}{dx} (6x) = 6 \cdot 1x^{1-1} = 6
   \]
4. **Differentiate \( -7 \) (a constant)**:
   \[
   \frac{d}{dx} (-7) = 0
   \]

**Step 2: Combine the Results**
\[
f'(x) = 12x^2 - 10x + 6
\]

**Final Answer:**
\[
\mathbf{f'(x) = 12x^2 - 10x + 6}
\]

This confirms that the derivative is **\( 12x^2 - 10x + 6 \)**. üöÄ

  </br>

</details>

</br>

##### 7. Determine the local minima and maxima of the function f(x) = x^3^ 6x^2^ + 9x

<details>
  <summary>Solution</summary>

To determine the **local minima and maxima** of the function:

\[
f(x) = x^3 + 6x^2 + 9x
\]

we follow these steps:

**Step 1: Find the First Derivative \( f'(x) \)**
Differentiate the function:

\[
f'(x) = \frac{d}{dx} (x^3 + 6x^2 + 9x)
\]

Using the **power rule**:

\[
f'(x) = 3x^2 + 12x + 9
\]

**Step 2: Find Critical Points**
Set \( f'(x) = 0 \) to find critical points:

\[
3x^2 + 12x + 9 = 0
\]

Divide by 3:

\[
x^2 + 4x + 3 = 0
\]

Factorize:

\[
(x+3)(x+1) = 0
\]

Solve for \( x \):

\[
x = -3, \quad x = -1
\]

These are the **critical points**.
**Step 3: Find the Second Derivative \( f''(x) \)**
Differentiate \( f'(x) \):

\[
f''(x) = \frac{d}{dx} (3x^2 + 12x + 9)
\]

\[
f''(x) = 6x + 12
\]

**Step 4: Determine the Nature of Critical Points**
Use the **second derivative test**:

- **At \( x = -3 \):**
  \[
  f''(-3) = 6(-3) + 12 = -18 + 12 = -6
  \]
  Since \( f''(-3) < 0 \), **\( x = -3 \) is a local maximum**.

- **At \( x = -1 \):**
  \[
  f''(-1) = 6(-1) + 12 = -6 + 12 = 6
  \]
  Since \( f''(-1) > 0 \), **\( x = -1 \) is a local minimum**.
  **Step 5: Find Function Values**
  To determine the actual maximum and minimum values:

- **At \( x = -3 \):**
  \[
  f(-3) = (-3)^3 + 6(-3)^2 + 9(-3)
  \]
  \[
  = -27 + 6(9) + (-27) = -27 + 54 - 27 = 0
  \]

- **At \( x = -1 \):**
  \[
  f(-1) = (-1)^3 + 6(-1)^2 + 9(-1)
  \]
  \[
  = -1 + 6(1) + (-9) = -1 + 6 - 9 = -4
  \]

**Final Answer**

- **Local Maximum at \( x = -3 \) with \( f(-3) = 0 \)**
- **Local Minimum at \( x = -1 \) with \( f(-1) = -4 \)**

üöÄ **Summary:**

- **Local Max:** \( (-3, 0) \)
- **Local Min:** \( (-1, -4) \)

  </br>

</details>

</br>
