#### Limits and differentiation - summative quiz

##### 1. What is the value of lim~x->2~ ${\frac{x^2 - 4}{x-2}}$

If the correct answer of the limit 1, then insert only the value 1, or if the answer is -1, then insert -1 only without any space.

<details>
  <summary>Solution</summary>

To evaluate the limit:

\[
\lim\_{{x \to 2}} \frac{x^2 - 4}{x - 2}
\]

**Step 1: Factor the Numerator**
The numerator can be factored as:

\[
x^2 - 4 = (x - 2)(x + 2)
\]

So the given limit simplifies to:

\[
\lim\_{{x \to 2}} \frac{(x - 2)(x + 2)}{x - 2}
\]

**Step 2: Cancel the Common Factor**
For \( x \neq 2 \), we can cancel \( (x - 2) \):

\[
\lim\_{{x \to 2}} x + 2
\]

**Step 3: Substitute \( x = 2 \)**
\[
2 + 2 = 4
\]
**Final Answer:**
\[
4
\]

  </br>

</details>

</br>

##### 2. Calculate the value of the following limit:

lim~x->2~ f(x) = ${\frac{x^2+4x-12}{x^2-2x}}$

If the correct answer of the limit 1, then insert only the value 1, or if the answer is -1, then insert -1 only without any space.

<details>
  <summary>Solution</summary>

To evaluate the limit:

\[
\lim\_{{x \to 2}} \frac{x^2 + 4x - 12}{x^2 - 2x}
\]

**Step 1: Factor the Numerator and Denominator**

- Factor the numerator \( x^2 + 4x - 12 \):

\[
x^2 + 4x - 12 = (x + 6)(x - 2)
\]

- Factor the denominator \( x^2 - 2x \):

\[
x^2 - 2x = x(x - 2)
\]

Now, the expression becomes:

\[
\frac{(x + 6)(x - 2)}{x(x - 2)}
\]

**Step 2: Cancel the Common Factor**
For \( x \neq 2 \), cancel \( (x - 2) \):

\[
\frac{x + 6}{x}
\]

**Step 3: Substitute \( x = 2 \)**
\[
\frac{2 + 6}{2} = \frac{8}{2} = 4
\]
**Final Answer:**
\[
4
\]

  </br>

</details>

</br>

##### 3. What is the limit of the function lim~x->5~ f(x) ${\frac{x^2+3x-10}{x+5}}$

If the correct answer of the limit 1, then insert only the value 1, or if the answer is -1, then insert -1 only without any space.

<details>
  <summary>Solution</summary>

To evaluate:

\[
\lim\_{{x \to 5}} \frac{x^2 + 3x - 10}{x + 5}
\]

**Step 1: Factor the Numerator**
The numerator \( x^2 + 3x - 10 \) can be factored:

\[
x^2 + 3x - 10 = (x - 2)(x + 5)
\]

So the function becomes:

\[
\frac{(x - 2)(x + 5)}{x + 5}
\]

**Step 2: Cancel the Common Factor**
For \( x \neq -5 \), we can cancel \( (x + 5) \):

\[
f(x) = x - 2
\]
**Step 3: Substitute \( x = 5 \)**
\[
f(5) = 5 - 2 = 3
\]

**Final Answer:**
\[
3
\]

Since the result is **not 1 or -1**, I will not insert any value. ðŸš€

  </br>

</details>

</br>
